

Tutorial of Hopfield Network

A binary Hopfield network is used to store 4 binary 4-dimensional patterns, $x_1 = [1, 1, -1, -1]$, $x_2 = [-1, -1, 1, 1]$, $x_3 = [-1, 1, 1, -1]$ and $x_4 = [1, 1, 1, -1]$.

1. Compute the weight matrix W for the Hopfield network.
2. Recover the value of the 2nd dimension when the input state is $x_5 = [1, ?, -1, -1]$
3. Given a noisy input $[1, -1, 1, -1]$, using asynchronous mode update rule to determine the final stable state of the network (node selection sequence is $1 > 2 > 3 > 4$).
4. Assuming we use a Hopfield network with no external inputs, please answer

Question 3 again.

$$\begin{aligned}
 1. \quad W &= \frac{1}{N} \sum_{p=1}^P x^p x^{pT} - \theta I \\
 &= \frac{1}{4} \begin{bmatrix} 1 \\ 1 \\ -1 \\ -1 \end{bmatrix} \begin{bmatrix} 1 & 1 & -1 & -1 \end{bmatrix} - 4I \\
 &\quad + x_2 x_2^T + x_3 x_3^T + x_4 x_4^T
 \end{aligned}$$

Answer:

Q1. Let I denotes identity matrix, the the weight matrix W is computed as the followed equation:

$$W = \frac{1}{N} \sum_{n=1, \dots, N} x_n x_n^T - I$$

or the element of the weight matrix W is computed as:

$$w_{ij} = \begin{cases} \frac{1}{N} \sum_{n=1, \dots, N} x_n(i) x_n(j) & \text{if } i \neq j \\ 0, & \text{if } i = j \end{cases}$$

$w_{12} = \frac{1}{4} x_1 \cdot x_2$
=

And both the following to calculating method, (1) and (2), are correct.

a.

$$x_1 x_1^T = \begin{bmatrix} 1 & 1 & -1 & -1 \\ 1 & 1 & -1 & -1 \\ -1 & -1 & 1 & 1 \\ -1 & -1 & 1 & 1 \end{bmatrix}$$

$$x_2 x_2^T = \begin{bmatrix} 1 & 1 & -1 & -1 \\ 1 & 1 & -1 & -1 \\ -1 & -1 & 1 & 1 \\ -1 & -1 & 1 & 1 \end{bmatrix}$$

$$x_3 x_3^T = \begin{bmatrix} 1 & -1 & -1 & 1 \\ -1 & 1 & 1 & -1 \\ -1 & 1 & 1 & -1 \\ 1 & -1 & -1 & 1 \end{bmatrix}$$

$$x_4 x_4^T = \begin{bmatrix} 1 & 1 & 1 & -1 \\ 1 & 1 & 1 & -1 \\ 1 & 1 & 1 & -1 \\ -1 & -1 & -1 & 1 \end{bmatrix}$$

$w_{12} = \frac{1}{4} \sum_{n=1}^4 x_n(1) x_n(2)$
 $= \frac{1}{4} (1 + 1 - 1 + 1)$
 $w_{13} = \frac{1}{4} (-1 - 1 - 1 + 1)$

According the equation, the weight matrix is given:

$$W = \frac{1}{4} \begin{bmatrix} 0 & 2 & -2 & -2 \\ 2 & 0 & 0 & -4 \\ -2 & 0 & 0 & 0 \\ -2 & -4 & 0 & 0 \end{bmatrix}$$

b.

$$w_{11} = w_{22} = w_{33} = w_{44} = 0$$

$$w_{12} = w_{21} = \frac{1}{4}(1 + 1 - 1 + 1) = 2/4$$

$$w_{13} = w_{31} = \frac{1}{4}(-1 - 1 - 1 + 1) = \frac{-2}{4}$$

$$w_{14} = w_{41} = \frac{1}{4}(-1 - 1 + 1 - 1) = -2/4$$

$$w_{23} = w_{32} = \frac{1}{4}(-1 - 1 + 1 + 1) = 0$$

$$w_{24} = w_{42} = \frac{1}{4}(-1 - 1 - 1 - 1) = -4/4$$

$$w_{34} = w_{43} = \frac{1}{4}(1 + 1 - 1 - 1) = 0$$

Handwritten calculations and notes:

- $\frac{2}{4} + \frac{6}{4}$
- $\frac{2}{4} \times 1$
- 0×-1
- $\frac{1}{4} \times 1$
- w_{21} with $n=1$
- w_{23} with $n=3$
- w_{24} with $n=4$

Q2. The update rule for each missing dimension is given by:

$$y^j(t+1) = \sum_{n=1, n \neq j}^4 w_{jn} x^n(t)$$

$$x^j(t+1) = \text{sgn}(y^j(t+1)) = \begin{cases} 1, & \text{if } y^j(t+1) \geq 0 \\ -1, & \text{if } y^j(t+1) < 0 \end{cases}$$

Therefore: $y^2(0) = \frac{1}{4} (2 \cdot 1 + 0 \cdot (-1) + (-4) \cdot (-1) + (0)) = 6/4$

$$x^5(0) = \text{sgn}(y^2(0)) = 1$$

Q3. The update rule for each dimension is given by:

$$y^j(t+1) = \sum_{n=1, n \neq j}^4 w_{jn} x^n(t) + I_j$$

$$x^j(t+1) = \text{sgn}(y^j(t+1)) = \begin{cases} 1, & \text{if } y^j(t+1) \geq 0 \\ -1, & \text{if } y^j(t+1) < 0 \end{cases}$$

1 node: $y^1(0) = \frac{1}{4} (2*(-1)+(-2)*(1)+(-2)*(-1))+1 = 2/4$

$$x^1(0) = \text{sgn}(y^1(0)) = 1$$

2 node: $y^2(0) = \frac{1}{4} (2*1+0*(1)+(-4)*(-1))+(-1) = 2/4$

$$x^2(0) = \text{sgn}(y^2(0)) = 1$$

3 node: $y^3(0) = \frac{1}{4} ((-2*1)+0*(1)+(0)*(-1))+1 = 2/4$

$$x^3(0) = \text{sgn}(y^3(0)) = 1$$

4 node: $y^4(0) = \frac{1}{4} ((-2)*1+(-4)*(1)+(0)*(1))+(-1) = -10/4$

$$x^4(0) = \text{sgn}(y^4(0)) = -1$$

Q4. As there is no any external input, the update rule for each dimension is given by:

$$y^j(t+1) = \sum_{n=1, n \neq j}^4 w_{jn} x^n(t)$$

$$x^j(t+1) = \text{sgn}(y^j(t+1)) = \begin{cases} 1, & \text{if } y^j(t+1) \geq 0 \\ -1, & \text{if } y^j(t+1) < 0 \end{cases}$$

1 node: $y^1(0) = \frac{1}{4} (2*(-1)+(-2)*(1)+(-2)*(-1)) = -2/4$

$$x^1(0) = \text{sgn}(y^1(0)) = -1$$

2 node: $y^2(0) = \frac{1}{4} (2*(-1)+0*(1)+(-4)*(-1)) = 2/4$

$$x^2(0) = \text{sgn}(y^2(0)) = 1$$

3 node: $y^3(0) = \frac{1}{4} ((-2)*(-1)+0*(1)+(0)*(-1)) = 2/4$

$$x^3(0) = \text{sgn}(y^3(0)) = 1$$

4 node: $y^4(0) = \frac{1}{4} ((-2)*(-1)+(-4)*(1)+(0)*(1)) = -2/4$

$$x^4(0) = \text{sgn}(y^4(0)) = -1$$